updated bitvector library

theories/bitvector.v
@@ -1,74 +1,115 @@
-Require Export isla.base.
+From stdpp Require Export numbers.
+From stdpp Require Import countable.
+From stdpp Require Import options.
 
+Local Open Scope Z_scope.
+
+Lemma pos_bounded_iff_bits k n :
+  (0 ≤ k → 0 ≤ n → n < 2^k ↔ ∀ l, k ≤ l → Z.testbit n l = false)%Z.
+Proof.
+  intros.
+  destruct (decide (n = 0)) as [->|].
+  - setoid_rewrite Z.bits_0. split; [done|]. intros. by apply Z.pow_pos_nonneg.
+  - split.
+    + intros Hb%Z.log2_lt_pow2 l Hl; [| lia]. apply Z.bits_above_log2; lia.
+    + intros Hl.
+      destruct (decide (n < 2^k)%Z); [done|].
+      assert (Z.testbit n (Z.log2 n) = false) as Hbit.
+      { apply Hl, Z.log2_le_pow2; lia. }
+      rewrite Z.bit_log2 in Hbit; [done| lia].
+Qed.
+
+
+(*** Preliminary definitions *)
+Definition bv_modulus (n : N) : Z := 2 ^ (Z.of_N n).
+Definition bv_half_modulus (n : N) : Z := 2 ^ (Z.of_N (n - 1)).
+Definition bv_wrap (n : N) (z : Z) : Z := z `mod` bv_modulus n.
+Definition bv_swrap (n : N) (z : Z) : Z := bv_wrap n (z + bv_half_modulus n) - bv_half_modulus n.
+Definition bv_ok (n : N) (z : Z) : Prop := -1 < z < bv_modulus n.
+
+Lemma bv_modulus_pos n :
+  0 < bv_modulus n.
+Proof. apply Z.pow_pos_nonneg; lia. Qed.
+
+Lemma bv_modulus_add n1 n2 :
+  bv_modulus (n1 + n2) = bv_modulus n1 * bv_modulus n2.
+Proof. unfold bv_modulus. rewrite N2Z.inj_add. eapply Z.pow_add_r; lia. Qed.
+
+Lemma bv_ok_in_range n z:
+  bv_ok n z ↔ 0 ≤ z < bv_modulus n.
+Proof. unfold bv_ok. lia. Qed.
+
+Lemma bv_wrap_ok n z :
+  bv_ok n (bv_wrap n z).
+Proof.
+  unfold bv_wrap.
+  pose proof (Z.mod_pos_bound z (bv_modulus n)) as [??]. { apply bv_modulus_pos. }
+  split; lia.
+Qed.
+
+Lemma bv_ok_bitwise_op {n} op bop n1 n2 :
+  (∀ k, Z.testbit (op n1 n2) k = bop (Z.testbit n1 k) (Z.testbit n2 k)) →
+  (0 ≤ n1 → 0 ≤ n2 → 0 ≤ op n1 n2) →
+  bop false false = false →
+  bv_ok n n1 → bv_ok n n2 → bv_ok n (op n1 n2).
+Proof.
+  intros Hbits Hnonneg Hop [? Hok1]%bv_ok_in_range [? Hok2]%bv_ok_in_range. apply bv_ok_in_range.
+  split; [lia|].
+  apply pos_bounded_iff_bits; [lia..|]. intros l ?.
+  eapply pos_bounded_iff_bits in Hok1;[|try done; lia..].
+  eapply pos_bounded_iff_bits in Hok2;[|try done; lia..].
+  by rewrite Hbits, Hok1, Hok2.
+Qed.
+
+(*** Definition of [bv n] *)
 Record bv (n : N) := BV {
-  bv_val : Z;
-  bv_in_range : -1 < bv_val < 2 ^ Z.of_N n;
-  (* TODO: Should we include the above?
-  Arguments for:
-  - all bit vectors are in normal form by construction and equivalence becomes eq
-    - can maybe be mitigated by normalizing aggressively
-  Arguments against:
-  - Makes constants annoying to write (needs tactics in terms which seems to break stuff in weird ways, e.g typeclass search)
-  - n1 = n2 cannot be long solved by done
-  *)
+  bv_unsigned : Z;
+  bv_is_ok : bv_ok n bv_unsigned;
 }.
-Arguments bv_val {_}.
+Arguments bv_unsigned {_}.
+Arguments bv_is_ok {_}.
+
+Definition bv_signed {n} (b : bv n) := bv_swrap n (bv_unsigned b).
+
+Lemma bv_eq n (b1 b2 : bv n) :
+  b1 = b2 ↔ b1.(bv_unsigned) = b2.(bv_unsigned).
+Proof. destruct b1, b2. split; simpl; [ naive_solver|]. intros. subst. f_equal. apply proof_irrel. Qed.
 
 Global Program Instance bv_eq_dec n : EqDecision (bv n) := λ '(BV _ v1 p1) '(BV _ v2 p2),
    match decide (v1 = v2) with
    | left eqv => left _
    | right eqv => right _
    end.
-Next Obligation. move => *. subst. f_equal. apply: proof_irrel. Qed.
-Next Obligation. move => * [?]. done. Qed.
+Next Obligation. intros. subst. rewrite (proof_irrel p1 p2). exact eq_refl. Defined.
+Next Obligation. intros. by injection. Qed.
 
-Lemma bv_eq n (b1 b2 : bv n) :
-  b1 = b2 ↔ b1.(bv_val) = b2.(bv_val).
-Proof. destruct b1, b2. split => /=; first by case. move => ?. subst. f_equal => //. apply: proof_irrel. Qed.
+Global Instance bv_countable n : Countable (bv n).
+Proof.
+  refine (inj_countable bv_unsigned
+    (λ x, match decide (bv_ok n x) with | left b => Some (BV n x b) | _ => None end) _).
+  intros x. case_decide; [ f_equal; by apply bv_eq|].
+  by pose proof bv_is_ok x.
+Qed.
 
-Coercion bv_val : bv >-> Z.
 
 Definition bv_of_Z_checked (n : N) (z : Z) : option (bv n) :=
-  match decide (-1 < z < 2 ^ Z.of_N n) with
+  match decide (bv_ok n z) with
   | left Heq => Some (BV n z Heq)
   | right _ => None
   end.
 
-Record bvn := BVN {
-  bvn_n : N;
-  bvn_val : bv bvn_n;
-}.
+Program Definition bv_of_Z (n : N) (z : Z) : bv n := {|
+  bv_unsigned := bv_wrap n z;
+|}.
+Next Obligation. apply bv_wrap_ok. Qed.
+Arguments bv_of_Z : simpl never.
+Global Opaque bv_of_Z.
 
-Lemma bvn_eq (b1 b2 : bvn) :
-  b1 = b2 ↔ b1.(bvn_n) = b2.(bvn_n) ∧ b1.(bvn_val).(bv_val) = b2.(bvn_val).(bv_val).
-Proof.
-  split; [ naive_solver|]. destruct b1, b2 => /= -[??]. subst. f_equal.
-  by apply/bv_eq.
-Qed.
+Lemma bv_in_range n (b : bv n):
+  0 ≤ bv_unsigned b < bv_modulus n.
+Proof. apply bv_ok_in_range. apply bv_is_ok. Qed.
 
-Global Program Instance bvn_eq_dec : EqDecision bvn := λ '(BVN n1 b1) '(BVN n2 b2),
-   match decide (n1 = n2) with
-   | left eqv => match decide (b1.(bv_val) = b2.(bv_val)) with
-                | left eqb => left _
-                | right eqb => right _
-                end
-   | right eqv => right _
-   end.
-Next Obligation. move => *. apply/bvn_eq. naive_solver. Qed.
-Next Obligation. move => *. apply/bvn_eq. naive_solver. Qed.
-Next Obligation. move => *. apply/bvn_eq. naive_solver. Qed.
-
-Definition bvn_to_bv (n : N) (b : bvn) : option (bv n) :=
-  match decide (b.(bvn_n) = n) with
-  | left eq => Some (eq_rect (bvn_n b) (λ n0 : N, bv n0)
-           (bvn_val b) n eq)
-  | right _ => None
-  end.
-Arguments bvn_to_bv !_ !_ /.
-
-Definition bv_to_bvn {n} (b : bv n) : bvn := BVN _ b.
-Coercion bv_to_bvn : bv >-> bvn.
-
+(*** Notation for [bv n] *)
 Ltac solve_bitvector_eq :=
   try (vm_compute; done);
   lazymatch goal with
@@ -77,77 +118,158 @@ Ltac solve_bitvector_eq :=
   end.
 
 Notation "'[BV{' l } v ]" := (BV l v _) (at level 9, format "[BV{ l }  v ]", only printing) : stdpp_scope.
+(* TODO: This notation breaks when used in gmap notations. Why? *)
 Notation "'[BV{' l } v ]" := (BV l v ltac:(solve_bitvector_eq)) (at level 9, only parsing) : stdpp_scope.
-(* Notation "'[BV{' l } v ]" := (BV l v) (at level 9, format "[BV{ l }  v ]") : stdpp_scope. *)
 
+(*** Automation *)
+(* From Program.Tactics *)
+Ltac add_hypothesis H' p :=
+  match type of p with
+    ?X =>
+    match goal with
+      | [ H : X |- _ ] => fail 1
+      | _ => set (H':=p) ; try (change p with H') ; clearbody H'
+    end
+  end.
+Ltac bv_saturate :=
+  repeat match goal with
+         | b : bv _ |- _ =>
+           let H := fresh in
+           add_hypothesis H (bv_in_range _ b)
+         end.
+
+
+(*** Operations on [bv n] *)
+
+Definition bv_add {n} (x y : bv n) : bv n := (* SMT: bvadd *)
+  bv_of_Z n (Z.add (bv_unsigned x) (bv_unsigned y)).
+Definition bv_sub {n} (x y : bv n) : bv n := (* SMT: bvsub *)
+  bv_of_Z n (Z.sub (bv_unsigned x) (bv_unsigned y)).
+Definition bv_opp {n} (x y : bv n) : bv n := (* SMT: bvneg *)
+  bv_of_Z n (Z.opp (bv_unsigned x)).
+
+Definition bv_mul {n} (x y : bv n) : bv n := (* SMT: bvmul *)
+  bv_of_Z n (Z.mul (bv_unsigned x) (bv_unsigned y)).
+Definition bv_divu {n} (x y : bv n) : bv n := (* SMT: bvudiv *)
+  bv_of_Z n (Z.div (bv_unsigned x) (bv_unsigned y)).
+Definition bv_modu {n} (x y : bv n) : bv n := (* SMT: bvurem *)
+  bv_of_Z n (Z.modulo (bv_unsigned x) (bv_unsigned y)).
+Definition bv_divs {n} (x y : bv n) : bv n :=
+  bv_of_Z n (Z.div (bv_signed x) (bv_signed y)).
+Definition bv_quots {n} (x y : bv n) : bv n := (* SMT: bvsdiv *)
+  bv_of_Z n (Z.quot (bv_signed x) (bv_signed y)).
+Definition bv_mods {n} (x y : bv n) : bv n := (* SMT: bvsmod *)
+  bv_of_Z n (Z.modulo (bv_signed x) (bv_signed y)).
+Definition bv_rems {n} (x y : bv n) : bv n := (* SMT: bvsrem *)
+  bv_of_Z n (Z.rem (bv_signed x) (bv_signed y)).
+
+Definition bv_shiftl {n} (x y : bv n) : bv n := (* SMT: bvshl *)
+  bv_of_Z n (Z.shiftl (bv_unsigned x) (bv_unsigned y)).
+Definition bv_shiftr {n} (x y : bv n) : bv n := (* SMT: bvlshr *)
+  bv_of_Z n (Z.shiftr (bv_unsigned x) (bv_unsigned y)).
+Definition bv_ashiftr {n} (x y : bv n) : bv n := (* SMT: bvashr *)
+  bv_of_Z n (Z.shiftr (bv_signed x) (bv_unsigned y)).
+
+Program Definition bv_or {n} (x y : bv n) : bv n := (* SMT: bvor *)
+  BV n (Z.lor (bv_unsigned x) (bv_unsigned y)) _.
+Next Obligation.
+  intros. eapply bv_ok_bitwise_op; [ apply Z.lor_spec | by intros; eapply Z.lor_nonneg | done | apply bv_is_ok..].
+Qed.
+Program Definition bv_and {n} (x y : bv n) : bv n := (* SMT: bvand *)
+  BV n (Z.land (bv_unsigned x) (bv_unsigned y)) _.
+Next Obligation.
+  intros. eapply bv_ok_bitwise_op; [ apply Z.land_spec | intros; eapply Z.land_nonneg; by left | done | apply bv_is_ok..].
+Qed.
+Program Definition bv_xor {n} (x y : bv n) : bv n := (* SMT: bvxor *)
+  BV n (Z.lxor (bv_unsigned x) (bv_unsigned y)) _.
+Next Obligation.
+  intros. eapply bv_ok_bitwise_op; [ apply Z.lxor_spec | intros; eapply Z.lxor_nonneg; naive_solver | done | apply bv_is_ok..].
+Qed.
+Program Definition bv_not {n} (x : bv n) : bv n := (* SMT: bvnot *)
+  bv_of_Z n (Z.lnot (bv_unsigned x)).
+
+Program Definition bv_zero_extend {n} (z : N) (b : bv n) : bv (n + z) := (* SMT: zero_extend *)
+  BV _ (bv_unsigned b) _.
+Next Obligation.
+  intros. apply bv_ok_in_range. rewrite bv_modulus_add. bv_saturate.
+  pose proof (bv_modulus_pos z). nia.
+Qed.
+
+Program Definition bv_sign_extend {n} (z : N) (b : bv n) : bv (n + z) := (* SMT: sign_extend *)
+  bv_of_Z _ (bv_signed b).
+
+(* s is start index and l is length. Note that this is different from
+extract in SMTLIB which uses [extract (inclusive upper bound)
+(inclusive lower bound)] *)
+Program Definition bv_extract {n} (s l : N) (b : bv n) : bv l :=
+  BV l (Z.land (bv_unsigned b ≫ Z.of_N s) (Z.ones (Z.of_N l))) _.
+Next Obligation.
+  intros.
+  apply bv_ok_in_range.
+  assert (0 ≤ Z.land (bv_unsigned b ≫ Z.of_N s) (Z.ones (Z.of_N l))).
+  { apply Z.land_nonneg. left. apply Z.shiftr_nonneg. bv_saturate. lia. }
+  split; [lia|]. apply pos_bounded_iff_bits; [lia.. |].
+  intros k ?. rewrite Z.land_spec. apply andb_false_intro2.
+  apply Z.ones_spec_high. lia.
+Qed.
+
+Program Definition bv_concat {n1 n2} (b1 : bv n1) (b2 : bv n2) : bv (n1 + n2) := (* SMT: concat *)
+  BV _ (Z.lor (bv_unsigned b1 ≪ Z.of_N n2) (bv_unsigned b2)) _.
+Next Obligation.
+  intros.
+  apply bv_ok_in_range.
+  assert (0 ≤ Z.lor (bv_unsigned b1 ≪ Z.of_N n2) (bv_unsigned b2)).
+  { apply Z.lor_nonneg. bv_saturate. split; [|lia]. apply Z.shiftl_nonneg. lia. }
+  split; [lia|]. apply pos_bounded_iff_bits; [lia.. |].
+  intros k ?. rewrite Z.lor_spec, Z.shiftl_spec; [|lia].
+  apply orb_false_intro; (eapply pos_bounded_iff_bits; [..|done]); bv_saturate; try lia.
+  - apply (Z.lt_le_trans _ (bv_modulus n1)); [lia|]. apply Z.pow_le_mono_r; lia.
+  - apply (Z.lt_le_trans _ (bv_modulus n2)); [lia|]. apply Z.pow_le_mono_r; lia.
+Qed.
+
+(*** [bvn] *)
+Record bvn := BVN {
+  bvn_n : N;
+  bvn_val : bv bvn_n;
+}.
+
+Definition bvn_unsigned (b : bvn) := bv_unsigned (b.(bvn_val)).
+
+Lemma bvn_eq (b1 b2 : bvn) :
+  b1 = b2 ↔ b1.(bvn_n) = b2.(bvn_n) ∧ bvn_unsigned b1 = bvn_unsigned b2.
+Proof. split; [ naive_solver|]. destruct b1, b2; simpl; intros [??]. subst. f_equal. by apply bv_eq. Qed.
+
+Global Program Instance bvn_eq_dec : EqDecision bvn := λ '(BVN n1 b1) '(BVN n2 b2),
+   match decide (n1 = n2) with
+   | left eqv => match decide (bv_unsigned b1 = bv_unsigned b2) with
+                | left eqb => left _
+                | right eqb => right _
+                end
+   | right eqv => right _
+   end.
+(* TODO: The following does not compute to eq_refl*)
+Next Obligation. intros. apply bvn_eq. naive_solver. Qed.
+Next Obligation. intros. intros ?%bvn_eq. naive_solver. Qed.
+Next Obligation. intros. intros ?%bvn_eq. naive_solver. Qed.
+
+Definition bvn_to_bv (n : N) (b : bvn) : option (bv n) :=
+  match decide (b.(bvn_n) = n) with
+  | left eq => Some (eq_rect (bvn_n b) (λ n0 : N, bv n0) (bvn_val b) n eq)
+  | right _ => None
+  end.
+Arguments bvn_to_bv !_ !_ /.
+
+Definition bv_to_bvn {n} (b : bv n) : bvn := BVN _ b.
+Coercion bv_to_bvn : bv >-> bvn.
+
+(*** [tests] *)
+Section test.
 Goal ([BV{10} 3 ] = [BV{10} 5]). Abort.
 Fail Goal ([BV{2} 3 ] = [BV{10} 5]).
 Goal ([BV{2} 3 ] =@{bvn} [BV{10} 5]). Abort.
 Fail Goal ([BV{2} 4 ] = [BV{2} 5]).
 Goal bvn_to_bv 2 [BV{2} 3] = Some [BV{2} 3]. done. Abort.
-
-
-Program Definition bv_zero_extend {n} (z : N) (b : bv n) : bv (n + z) := {|
-  bv_val := b.(bv_val);
-|}.
-Next Obligation. Admitted.
-
-Definition Z_to_signed (bits n : Z) : Z :=
-  if bool_decide (2 ^ (bits - 1) ≤ n) then
-    n - 2 ^ bits
-  else
-    n.
-
-Definition Z_to_unsigned (bits n : Z) : Z :=
-  if bool_decide (n ≤ 0) then
-    n + 2 ^ bits
-  else
-    n.
-
-Program Definition bv_sign_extend {n} (z : N) (b : bv n) : bv (n + z) := {|
-  bv_val := Z_to_unsigned (Z.of_N (n + z)) (Z_to_signed (Z.of_N n) b.(bv_val))
-|}.
-Next Obligation. Admitted.
-
-
-(* s is start, l is len *)
-Program Definition bv_extract {n} (s l : N) (b : bv n) : bv (l) := {|
-  bv_val := Z.land (b.(bv_val) ≫ Z.of_N s) (Z.ones (Z.of_N l));
-|}.
-Next Obligation. Admitted.
-
-Program Definition bv_add {n} (b1 b2 : bv n) : bv n := {|
-  bv_val := b1.(bv_val) + b2.(bv_val) `mod` 2 ^ Z.of_N n;
-|}.
-Next Obligation. Admitted.
-
-Program Definition bv_or {n} (n1 n2 : bv n) : bv n := {|
-  bv_val := Z.lor n1.(bv_val) n2.(bv_val);
-|}.
-Next Obligation. Admitted.
-
-Program Definition bv_and {n} (n1 n2 : bv n) : bv n := {|
-  bv_val := Z.land n1.(bv_val) n2.(bv_val);
-|}.
-Next Obligation. Admitted.
-
-Program Definition bv_not {n} (b : bv n) : bv n := {|
-  bv_val := Z_lunot (Z.of_N n) b.(bv_val);
-|}.
-Next Obligation. Admitted.
-
-Program Definition bv_concat {n1 n2} (b1 : bv n1) (b2 : bv n2) : bv (n1 + n2) := {|
-  (* TODO: Is this the right way around? *)
-  bv_val := Z.lor (b1.(bv_val) ≪ Z.of_N n2) b2.(bv_val);
-|}.
-Next Obligation. Admitted.
-
-Program Definition bv_shr {n} (n1 n2 : bv n) : bv n := {|
-  (* TODO: Is this the right way around? *)
-  bv_val := (n1.(bv_val) ≫ n2.(bv_val));
-|}.
-Next Obligation. Admitted.
-
+End test.
 
 (*
 (*** Old definition of bit vectors *)
